Loop

Extension1.v
@@ -1,18 +1,361 @@
 Set Warnings "-notation-overridden,-parsing".
 
+From Coq Require Import Bool.Bool.
+From Coq Require Import Init.Nat.
+From Coq Require Import Arith.Arith.
+From Coq Require Import Arith.EqNat.
+From Coq Require Import omega.Omega.
+From Coq Require Import Lists.List.
+From Coq Require Import Strings.String.
+Import ListNotations.
 
-(*D:\Development\Coq\plf\common was previously bound to PLF.common; it is remapped to common
-[overriding-logical-loadpath,loadpath]
-D:\Development\Coq\plf\common\css was previously bound to PLF.common.css; it is remapped to common.css
-[overriding-logical-loadpath,loadpath]
-D:\Development\Coq\plf\common\media was previously bound to PLF.common.media; it is remapped to common.media
-[overriding-logical-loadpath,loadpath]
-D:\Development\Coq\plf\common\media\font was previously bound to PLF.common.media.font; it is remapped to
-common.media.font [overriding-logical-loadpath,loadpath]
-D:\Development\Coq\plf\common\media\image was previously bound to PLF.common.media.image; it is remapped to
-common.media.image [overriding-logical-loadpath,loadpath]
-D:\Development\Coq\plf was previously bound to PLF; it is remapped to <> [overriding-logical-loadpath,loadpath]*)
+(*MAPS *)
+Definition total_map (A : Type) := string -> A.
 
-Add LoadPath "D:\Development\Coq\plf".
+Definition t_empty {A : Type} (v : A) : total_map A :=
+  (fun _ => v).
 
-Require Import Imp.
+
+
+Definition eqb_string (x y : string) : bool :=
+  if string_dec x y then true else false.
+
+Definition t_update {A : Type} (m : total_map A)
+                    (x : string) (v : A) :=
+  fun x' => if eqb_string x x' then v else m x'.
+
+Notation "'_' '!->' v" := (t_empty v)
+  (at level 100, right associativity).
+
+Notation "x '!->' v ';' m" := (t_update m x v)
+                              (at level 100, v at next level, right associativity).
+
+Definition empty_st := (_ !-> 0).
+
+(*imp*)
+Inductive aexp : Type :=
+  | ANum (n : nat)
+  | AId (x : string)              (* <--- NEW *)
+  | APlus (a1 a2 : aexp)
+  | AMinus (a1 a2 : aexp)
+  | AMult (a1 a2 : aexp).
+
+Inductive bexp : Type :=
+  | BTrue
+  | BFalse
+  | BEq (a1 a2 : aexp)
+  | BLe (a1 a2 : aexp)
+  | BNot (b : bexp)
+  | BAnd (b1 b2 : bexp).
+
+
+Definition state := total_map nat.
+
+Coercion AId : string >-> aexp.
+Coercion ANum : nat >-> aexp.
+
+Fixpoint aeval (st : state) (a : aexp) : nat :=
+  match a with
+  | ANum n => n
+  | AId x => st x                                (* <--- NEW *)
+  | APlus a1 a2 => (aeval st a1) + (aeval st a2)
+  | AMinus a1 a2  => (aeval st a1) - (aeval st a2)
+  | AMult a1 a2 => (aeval st a1) * (aeval st a2)
+  end.
+
+Fixpoint beval (st : state) (b : bexp) : bool :=
+  match b with
+  | BTrue       => true
+  | BFalse      => false
+  | BEq a1 a2   => (aeval st a1) =? (aeval st a2)
+  | BLe a1 a2   => (aeval st a1) <=? (aeval st a2)
+  | BNot b1     => negb (beval st b1)
+  | BAnd b1 b2  => andb (beval st b1) (beval st b2)
+  end.
+
+Definition bool_to_bexp (b : bool) : bexp :=
+  if b then BTrue else BFalse.
+Coercion bool_to_bexp : bool >-> bexp.
+
+Bind Scope imp_scope with aexp.
+Bind Scope imp_scope with bexp.
+Delimit Scope imp_scope with imp.
+
+
+
+Definition W : string := "W".
+Definition X : string := "X".
+Definition Y : string := "Y".
+Definition Z : string := "Z".
+
+Notation "x + y" := (APlus x y) (at level 50, left associativity) : imp_scope.
+Notation "x - y" := (AMinus x y) (at level 50, left associativity) : imp_scope.
+Notation "x * y" := (AMult x y) (at level 40, left associativity) : imp_scope.
+Notation "x <= y" := (BLe x y) (at level 70, no associativity) : imp_scope.
+Notation "x = y" := (BEq x y) (at level 70, no associativity) : imp_scope.
+Notation "x && y" := (BAnd x y) (at level 40, left associativity) : imp_scope.
+Notation "'~' b" := (BNot b) (at level 75, right associativity) : imp_scope.
+
+Inductive com : Type :=
+  | CSkip
+  | CAss (x : string) (a : aexp)
+  | CSeq (c1 c2 : com)
+  | CIf (b : bexp) (c1 c2 : com)
+  | CWhile (b : bexp) (c : com)
+  | CLoop (a : aexp) (c : com).
+
+
+Bind Scope imp_scope with com.
+Notation "'SKIP'" :=
+   CSkip : imp_scope.
+Notation "x '::=' a" :=
+  (CAss x a) (at level 60) : imp_scope.
+Notation "c1 ;; c2" :=
+  (CSeq c1 c2) (at level 80, right associativity) : imp_scope.
+Notation "'WHILE' b 'DO' c 'END'" :=
+  (CWhile b c) (at level 80, right associativity) : imp_scope.
+Notation "'TEST' c1 'THEN' c2 'ELSE' c3 'FI'" :=
+  (CIf c1 c2 c3) (at level 80, right associativity) : imp_scope.
+Notation "'LOOP' a 'DO' c 'END'" :=
+  (CLoop a c) (at level 70, right associativity) : imp_scope.
+
+Reserved Notation "st '=[' c ']=>' st'"
+                  (at level 40).
+
+Inductive ceval : com -> state -> state -> Prop :=
+  | E_Skip : forall st,
+      st =[ SKIP ]=> st
+  | E_Ass  : forall st a1 n x,
+      aeval st a1 = n ->
+      st =[ x ::= a1 ]=> (x !-> n ; st)
+  | E_Seq : forall c1 c2 st st' st'',
+      st  =[ c1 ]=> st'  ->
+      st' =[ c2 ]=> st'' ->
+      st  =[ c1 ;; c2 ]=> st''
+  | E_IfTrue : forall st st' b c1 c2,
+      beval st b = true ->
+      st =[ c1 ]=> st' ->
+      st =[ TEST b THEN c1 ELSE c2 FI ]=> st'
+  | E_IfFalse : forall st st' b c1 c2,
+      beval st b = false ->
+      st =[ c2 ]=> st' ->
+      st =[ TEST b THEN c1 ELSE c2 FI ]=> st'
+  | E_WhileFalse : forall b st c,
+      beval st b = false ->
+      st =[ WHILE b DO c END ]=> st
+  | E_WhileTrue : forall st st' st'' b c,
+      beval st b = true ->
+      st  =[ c ]=> st' ->
+      st' =[ WHILE b DO c END ]=> st'' ->
+      st  =[ WHILE b DO c END ]=> st''
+  | E_LoopZero : forall st a c,
+    a = 0 -> 
+    st =[ LOOP a DO c END ]=> st
+  | E_LoopMore : forall st st' st'' a c,
+    a > 0 ->
+    st =[ c ]=> st' -> 
+    st' =[ LOOP (pred a) DO c END ]=> st'' ->
+    st =[ LOOP a DO c END ]=> st''
+
+  where "st =[ c ]=> st'" := (ceval c st st').
+
+
+
+Example ex1: forall x c, (x) =[ LOOP 0 DO c END ]=> (x).
+
+Proof.
+  intros. apply E_LoopZero. reflexivity.
+Qed.
+
+Example ex2: (X !-> 0; empty_st) =[ LOOP 4 DO X ::= X + 1 END ]=> (X !-> 4; X !-> 3; X !-> 2; X !-> 1; X !-> 0; empty_st).
+
+Proof.
+  repeat 
+  (try (eapply E_LoopMore; try apply le_plus_l; try (apply E_Ass; reflexivity)); 
+  try (apply E_LoopZero; reflexivity)).
+Qed.
+
+(* TODO: We should probably try to prove that our rule doesn't break the other rules, as well as its general correctness *)
+
+Theorem ceval_deterministic: forall c st st1 st2,
+     st =[ c ]=> st1  ->
+     st =[ c ]=> st2 ->
+     st1 = st2.
+Proof.
+  intros c st st1 st2 E1 E2.
+  generalize dependent st2.
+  induction E1;
+           intros st2 E2; inversion E2; subst.
+  - (* E_Skip *) reflexivity.
+  - (* E_Ass *) reflexivity.
+  - (* E_Seq *)
+    assert (st' = st'0) as EQ1.
+    { (* Proof of assertion *) apply IHE1_1; assumption. }
+    subst st'0.
+    apply IHE1_2. assumption.
+  - (* E_IfTrue, b1 evaluates to true *)
+      apply IHE1. assumption.
+  - (* E_IfTrue,  b1 evaluates to false (contradiction) *)
+      rewrite H in H5. discriminate H5.
+  - (* E_IfFalse, b1 evaluates to true (contradiction) *)
+      rewrite H in H5. discriminate H5.
+  - (* E_IfFalse, b1 evaluates to false *)
+      apply IHE1. assumption.
+  - (* E_WhileFalse, b1 evaluates to false *)
+    reflexivity.
+  - (* E_WhileFalse, b1 evaluates to true (contradiction) *)
+    rewrite H in H2. discriminate H2.
+  - (* E_WhileTrue, b1 evaluates to false (contradiction) *)
+    rewrite H in H4. discriminate H4.
+  - (* E_WhileTrue, b1 evaluates to true *)
+      assert (st' = st'0) as EQ1.
+      { (* Proof of assertion *) apply IHE1_1; assumption. }
+      subst st'0.
+      apply IHE1_2. assumption.  
+  - reflexivity.
+  - Admitted.
+
+
+
+(* Hoare *)
+
+Definition Assertion := state -> Prop.
+
+Definition assert_implies (P Q : Assertion) : Prop :=
+  forall st, P st -> Q st.
+
+Notation "P ->> Q" := (assert_implies P Q)
+                      (at level 80) : hoare_spec_scope.
+Open Scope hoare_spec_scope.
+
+Notation "P <<->> Q" :=
+  (P ->> Q /\ Q ->> P) (at level 80) : hoare_spec_scope.
+
+Definition hoare_triple
+           (P : Assertion) (c : com) (Q : Assertion) : Prop :=
+  forall st st',
+     st =[ c ]=> st'  ->
+     P st  ->
+     Q st'.
+
+Notation "{{ P }}  c  {{ Q }}" :=
+  (hoare_triple P c Q) (at level 90, c at next level)
+  : hoare_spec_scope.
+
+
+Theorem hoare_post_true : forall (P Q : Assertion) c,
+  (forall st, Q st) ->
+  {{P}} c {{Q}}.
+Proof.
+  intros P Q c H. unfold hoare_triple.
+  intros st st' Heval HP.
+  apply H.  Qed.
+
+Theorem hoare_pre_false : forall (P Q : Assertion) c,
+  (forall st, ~ (P st)) ->
+  {{P}} c {{Q}}.
+Proof.
+  intros P Q c H. unfold hoare_triple.
+  intros st st' Heval HP.
+  unfold not in H. apply H in HP.
+  inversion HP.  Qed.
+
+Definition assn_sub X a P : Assertion :=
+  fun (st : state) =>
+    P (X !-> aeval st a ; st).
+
+Notation "P [ X |-> a ]" := (assn_sub X a P)
+  (at level 10, X at next level).
+
+
+Theorem hoare_asgn : forall Q X a,
+  {{Q [X |-> a]}} X ::= a {{Q}}.
+Proof.
+  unfold hoare_triple.
+  intros Q X a st st' HE HQ.
+  inversion HE. subst.
+  unfold assn_sub in HQ. assumption.  Qed.
+
+Theorem hoare_consequence_pre : forall (P P' Q : Assertion) c,
+  {{P'}} c {{Q}} ->
+  P ->> P' ->
+  {{P}} c {{Q}}.
+Proof.
+  intros P P' Q c Hhoare Himp.
+  intros st st' Hc HP. apply (Hhoare st st').
+  assumption. apply Himp. assumption. Qed.
+
+Theorem hoare_consequence_post : forall (P Q Q' : Assertion) c,
+  {{P}} c {{Q'}} ->
+  Q' ->> Q ->
+  {{P}} c {{Q}}.
+Proof.
+  intros P Q Q' c Hhoare Himp.
+  intros st st' Hc HP.
+  apply Himp.
+  apply (Hhoare st st').
+  assumption. assumption. Qed.
+
+Theorem hoare_consequence : forall (P P' Q Q' : Assertion) c,
+  {{P'}} c {{Q'}} ->
+  P ->> P' ->
+  Q' ->> Q ->
+  {{P}} c {{Q}}.
+Proof.
+  intros P P' Q Q' c Hht HPP' HQ'Q.
+  apply hoare_consequence_pre with (P' := P').
+  apply hoare_consequence_post with (Q' := Q').
+  assumption. assumption. assumption.  Qed.
+
+Theorem hoare_skip : forall P,
+     {{P}} SKIP {{P}}.
+Proof.
+  intros P st st' H HP. inversion H. subst.
+  assumption.  Qed.
+
+Theorem hoare_seq : forall P Q R c1 c2,
+     {{Q}} c2 {{R}} ->
+     {{P}} c1 {{Q}} ->
+     {{P}} c1;;c2 {{R}}.
+Proof.
+  intros P Q R c1 c2 H1 H2 st st' H12 Pre.
+  inversion H12; subst.
+  apply (H1 st'0 st'); try assumption.
+  apply (H2 st st'0); assumption. Qed.
+
+
+(*something ain't right here...
+Theorem hoare_loop : forall P e c t z st st',
+  {{fun _ => P st /\ (st t) = z /\ z > 0}} c;; t ::= t - 1 {{fun _ => P st' /\ st' t = (z - 1)}} ->
+  {{fun _ => P st /\ t = e}} LOOP e DO c END {{fun _ => P st' /\ (st' t) = 0}}.
+*)
+
+Theorem loop_trivial : forall P c e,
+  {{P}} c {{P}} -> 
+  {{P}} LOOP e DO c END {{P}}.
+
+(* | E_LoopZero : forall st a c,
+    a = 0 -> 
+    st =[ LOOP a DO c END ]=> st
+  | E_LoopMore : forall st st' st'' a c,
+    a > 0 ->
+    st =[ c ]=> st' -> 
+    st' =[ LOOP (pred a) DO c END ]=> st'' ->
+    st =[ LOOP a DO c END ]=> st''*)
+
+
+Proof.
+  intros. induction e.
+  - induction n. 
+  (* n = 0 *)  
+  + unfold hoare_triple. intros. remember 0 as a. apply (E_LoopZero st a c) in Heqa.
+  assert (Heq: st = st'). { apply ceval_deterministic with (CLoop a c) st. - apply Heqa. - apply H0. }
+  rewrite <- Heq. apply H1.
+  (* n > 0 *)  
+  + unfold hoare_triple. intros. unfold hoare_triple in IHn. unfold hoare_triple in H.
+  
+
+
+
+
+
